src/LamRefLogicFacts.v
@@ -1,0 +1,62 @@
+Require List.
+Import List.ListNotations.
+Require Import String.
+Require Import ZArith.
+
+Require Import src.LambdaRef.
+Require Import src.LamRefFacts.
+Require Import src.LambdaAssertions.
+
+Theorem triple_weaken (V : Set) (e : Expr V) P P' Q Q' :
+  sa_implies P' P ->
+  (forall v c, sa_implies (Q v c) (Q' v c)) ->
+  hoare_triple e P Q ->
+  hoare_triple e P' Q'.
+Proof.
+  unfold hoare_triple, sa_implies. eauto.
+Qed.
+
+Theorem triple_value (V : Set) (v : Value V) (P : StateAssertion V) :
+  hoare_triple v P (fun _ c => sa_star (sa_pure (c = 0)) P).
+Proof.
+  unfold hoare_triple, sa_star, sa_pure, sa_empty, disjoint_maps.
+  intros v' c m m' Hred. inversion Hred.
+  - intro p. repeat eexists; eauto.
+  - discriminate_red_Val.
+Qed.
+
+Theorem triple_value' (V : Set) (v : Value V) :
+  hoare_triple v sa_empty (fun _ c => sa_pure (c = 0)).
+Proof.
+  unfold hoare_triple, sa_pure, sa_empty.
+  intros v' c m m' Hred. inversion Hred.
+  - auto.
+  - discriminate_red_Val.
+Qed.
+
+Theorem triple_value_untimed (V : Set) (v : Value V) (P : StateAssertion V) :
+  hoare_triple v P (fun _ _ => P).
+Proof.
+  eapply triple_weaken; eauto using triple_value;
+    unfold sa_implies, sa_star, sa_pure, sa_empty;
+    [| intros v' c m [m1 [m2 [[? ?] [? [? ?]]]]]; subst ];
+    eauto.
+Qed.
+
+Theorem triple_lam (V : Set) (e : Expr _) (v : Value V) P Q :
+  hoare_triple (subst_e e v) P (fun v c => Q v (1+c)) ->
+  hoare_triple ((-\e) <* v) P Q.
+Proof.
+  unfold hoare_triple. intros Hhoare v' c m m' Hred. inversion Hred. subst.
+  eapply Hhoare. inversion H; subst; auto; discriminate_red_Val.
+Qed.
+
+Theorem triple_bneg (V : Set) (b : bool) :
+  @hoare_triple V ([~] (Bool b))
+    sa_empty
+    (fun v c => sa_pure (v = Bool (negb b) /\ c = 1)).
+Proof.
+  unfold hoare_triple, sa_pure, sa_empty. intros v c m m' Hred p.
+  inversion Hred. subst. inversion H; subst; try discriminate_red_Val.
+  inversion H0; subst; auto. discriminate_red_Val.
+Qed.
